Validator/Hedge/Types.lean
@@ -6,28 +6,12 @@ import Validator.Regex.Regex
 --   𝑇 a finite set of terminals
 --   𝑆 the start symbol of a regular hedge grammar is a regular expression comprising pairs of nonterminals and terminals (a regular expression over N × T)
 --   𝑃 a set of production rules of a regular hedge grammar are of the form X → r such that r is a regular expression over N × T.
+abbrev Ref (n: Nat) := Fin n
 
 namespace Hedge
 
 -- Ref is a non-terminal, where n represents the number of non-terminals
-abbrev Grammar.Ref (n: Nat) := Fin n
-
-abbrev Grammar.Symbol (n: Nat) (φ: Type) := (φ × Ref n)
-
-abbrev Grammar.Rule (n: Nat) (φ: Type) := Regex (Symbol n φ)
 
 structure Grammar (n: Nat) (φ: Type) where
-  start: Grammar.Rule n φ
-  prods: Vector (Grammar.Rule n φ) n
-
-end Hedge
-
-namespace Hedge.Grammar
-
-abbrev Symbols n φ l := Vector (Symbol n φ) l
-
-def hashVector [Hashable α] (xs: Vector α n): UInt64 :=
-  hash xs.toList
-
-instance (α: Type) (n: Nat) [Hashable α] : Hashable (Vector α n) where
-  hash := hashVector
+  start: Regex (φ × Ref n)
+  prods: Vector (Regex (φ × Ref n)) n
